src/termGen.ml
@@ -2,6 +2,7 @@ open Util
 open EConstr
 open TypeGen
 
+
 let get_constructor module_name constructor_name =
   let const_qualid = Libnames.qualid_of_string (if module_name != ""
                                                 then (String.concat "." [module_name; constructor_name])
