scratch/tjsoopsie.v
@@ -1,0 +1,903 @@
+Fixpoint free_vars (e:exp) (bound : list (ident string string)) : list (ident string string) :=
+  match e with
+  | ERaise e' => free_vars e' bound
+  | EHandle e' pes =>
+      free_vars e' bound ++
+                fold_right (@app (ident string string)) []
+                (map (fun '(p,e'') => free_vars e'' (map Short (pat_bindings p []))) pes)
+  | ELit _ => []
+  | ECon _ es => fold_right (@app (ident string string)) [] (map (fun e' => free_vars e' bound) es)
+  | EVar id => if existsb (fun i => ident_string_beq id i) bound then
+                []
+              else [id]
+  | EFun var e' => free_vars e' ((Short var)::bound)
+  | EApp _ es => fold_right (@app (ident string string)) [] (map (fun e' => free_vars e' bound) es)
+  | ELog _ e1 e2 => free_vars e1 bound ++ free_vars e2 bound
+  | EIf e0 e1 e2 => free_vars e0 bound ++ free_vars e1 bound ++ free_vars e2 bound
+  | EMat e' pes =>
+      free_vars e' bound ++
+                fold_right (@app (ident string string)) []
+                (map (fun '(p,e'') => free_vars e'' (map Short (pat_bindings p []))) pes)
+  | ELet None e1 e2 => free_vars e1 bound ++ free_vars e2 bound
+  | ELet (Some id) e1 e2 => free_vars e1 ((Short id)::bound) ++ free_vars e2 ((Short id)::bound)
+  | ELetrec funcs e' =>
+      let fun_names := map (fun '(fid,_,_) => Short fid) funcs in
+      free_vars e' (fun_names ++ bound) ++
+                fold_right (@app (ident string string)) []
+                (map (fun '(_,var,body) => free_vars body ((Short var)::(fun_names ++ bound))) funcs)
+  | ETannot e' _ | ELannot e' _ => free_vars e' bound
+  end.
+
+
+Fixpoint remove_dup_ids (ids : list (ident string string)) seen : list (ident string string) :=
+    match ids with
+    | [] => seen
+    | id::ids' => if existsb (fun i => ident_string_beq id i) seen
+                then remove_dup_ids ids' seen
+                else remove_dup_ids ids' (id::seen)
+    end.
+
+Fixpoint gather_values env_sev frees : env_val :=
+  match frees with
+  | [] => nsEmpty
+  | freev::frees' =>
+      match nsLookup ident_string_beq freev env_sev with
+      | None => gather_values env_sev frees'
+      | Some v => (freev,v)::(gather_values env_sev frees')
+      end
+  end.
+
+Definition optimize_recclosure_env (e : exp) (env : sem_env val) : sem_env val :=
+  let fvs := remove_dup_ids (free_vars e []) [] in
+  let env_sev := sev env in
+  update_sev env (gather_values env_sev fvs).
+
+From Equations Require Import Equations.
+Require Import StructTact.StructTactics.
+
+Lemma nsLookup_cover : forall V id x y (v : V),
+  nsLookup ident_string_beq id x = Some v ->
+  nsLookup ident_string_beq id (x ++ y) = Some v.
+Proof.
+  induction x; intros.
+  - inv H.
+  - unfold nsLookup in *. simpl in *.
+    destruct a.
+    break_if.
+    assumption.
+    apply IHx.
+    assumption.
+Qed.
+
+Lemma opti_somethin : forall id envv v fvs fvs',
+  nsLookup ident_string_beq id (gather_values envv fvs) = Some v ->
+  nsLookup ident_string_beq id (gather_values envv (fvs ++ fvs')) = Some v.
+Proof.
+  induction fvs; intros.
+  - inv H.
+  - simpl in *.
+    break_match.
+    unfold nsLookup in *. simpl in *.
+    break_if.
+    assumption.
+    apply IHfvs.
+    assumption.
+    apply IHfvs.
+    assumption.
+Qed.
+
+Lemma ident_string_beq_refl : forall id, ident_string_beq id id = true.
+Proof.
+  induction id.
+  - simpl.
+    apply eqb_refl.
+  - simpl.
+    rewrite eqb_refl.
+    rewrite IHid.
+    reflexivity.
+Qed.
+
+Lemma ident_string_beq_iff_false : forall id id', ident_string_beq id id' = false <-> id <> id'.
+Proof.
+  split;
+    generalize dependent id';
+    induction id; destruct id'; simpl.
+  - intros.
+    rewrite eqb_neq in H.
+    intro contra.
+    inv contra.
+    contradiction H. reflexivity.
+  - intros dc wrong. inv wrong.
+  - intros dc wrong. inv wrong.
+  - intros.
+    intro contra.
+    inversion contra.
+    eapply IHid.
+    rewrite H1 in H.
+    rewrite eqb_refl in H. simpl in H.
+    apply H.
+    apply H2.
+  - intro contra.
+    rewrite eqb_neq.
+    intro contra2.
+    contradiction contra.
+    subst. reflexivity.
+  - reflexivity.
+  - reflexivity.
+  - intros.
+    remember (x =? s) as fp.
+    destruct fp.
+    symmetry in Heqfp.
+    rewrite eqb_eq in Heqfp.
+    subst.
+    simpl.
+    apply IHid.
+    intro contra.
+    contradiction H.
+    subst; reflexivity.
+    reflexivity.
+Qed.
+
+Lemma ident_string_beq_iff_true : forall id id', ident_string_beq id id' = true <-> id = id'.
+Proof.
+  split;
+    generalize dependent id';
+    generalize dependent id;
+    induction id; destruct id'; intros; try inv H.
+  - simpl in H.
+    apply f_equal.
+    apply eqb_eq; assumption.
+  - rewrite Bool.andb_true_iff in H1.
+    destruct H1.
+    apply f_equal2.
+    rewrite eqb_eq in H0. assumption.
+    apply IHid.
+    assumption.
+  - apply ident_string_beq_refl.
+  - apply ident_string_beq_refl.
+Qed.
+
+Lemma ident_string_beq_sym : forall id id', ident_string_beq id id' = ident_string_beq id' id.
+Proof.
+  unfold ident_string_beq.
+  induction id; simpl.
+  destruct id'; simpl; try reflexivity.
+  apply eqb_sym.
+  destruct id'; simpl; try reflexivity.
+  rewrite IHid.
+  rewrite eqb_sym.
+  reflexivity.
+Qed.
+
+Lemma in_exists_eq : forall (A : Type) (eqb : A -> A -> bool) (a : A) l,
+    (forall x, eqb x x = true) ->
+    (forall x y, eqb x y = true <-> x = y) ->
+    existsb (fun a' => eqb a a') l = true <-> In a l.
+Proof.
+  split;
+    generalize dependent A.
+  - induction l.
+    + intros.
+      inv H1.
+    + intros.
+      simpl in *.
+      remember (eqb a a0) as eqa0.
+      destruct eqa0.
+      symmetry in Heqeqa0.
+      rewrite H0 in Heqeqa0.
+      symmetry in Heqeqa0.
+      left.
+      assumption.
+      simpl in *.
+      right.
+      apply IHl. assumption.
+      assumption.
+      assumption.
+  - induction l; intros.
+    + inv H1.
+    + simpl in H1.
+      destruct H1.
+      * simpl.
+        subst.
+        rewrite H.
+        reflexivity.
+      * simpl.
+        apply IHl in H1; try assumption.
+        rewrite H1. simpl.
+        apply Bool.orb_true_r.
+Qed.
+
+Lemma not_in_exists_eq : forall (A : Type) (eqb : A -> A -> bool) (a : A) l,
+    (forall x, eqb x x = true) ->
+    (forall x y, eqb x y = false <-> x <> y) ->
+    existsb (fun a' => eqb a a') l = false <-> ~ In a l.
+Proof.
+  split; generalize dependent A; induction l; intros.
+  - intro contra. inv contra.
+  - intro contra.
+    destruct contra. subst.
+    simpl in H1.
+    rewrite H in H1. inv H1.
+    simpl in H1.
+    rewrite Bool.orb_false_iff in H1.
+    destruct H1.
+    apply IHl; try assumption.
+  - reflexivity.
+  - simpl.
+    rewrite Bool.orb_false_iff.
+    assert (a <> a0).
+    intro contra.
+    apply H1.
+    left. subst. reflexivity.
+    split.
+    rewrite H0.
+    assumption.
+    apply IHl; try assumption.
+    intro contra.
+    contradiction H1.
+    right. assumption.
+Qed.
+
+Lemma idk_still : forall a l' l, In a l' -> remove_dup_ids (a::l) l' = remove_dup_ids l (l').
+Proof.
+  induction l'; intros.
+  - inv H.
+  - simpl in *.
+    destruct (Namespace.ident_eq_dec string string string_dec string_dec a0 a).
+    + subst. rewrite ident_string_beq_refl.
+      simpl. reflexivity.
+    + destruct H.
+      * apply n in H. contradiction H.
+      * rewrite <- ident_string_beq_iff_false in n.
+        rewrite ident_string_beq_sym.
+        rewrite n.
+        simpl.
+        rewrite <- in_exists_eq in H.
+        rewrite H.
+        reflexivity.
+        apply ident_string_beq_refl.
+        apply ident_string_beq_iff_true.
+Qed.
+
+Lemma opti_somethin''r : forall l l' a,
+    In a l' -> In a (remove_dup_ids l l').
+Proof.
+  induction l; intros.
+  - simpl. assumption.
+  - simpl.
+    remember (existsb (fun i => ident_string_beq a i) l') as thing.
+    destruct thing.
+    + apply IHl. assumption.
+    + apply IHl.
+      simpl. right. assumption.
+Qed.
+
+Lemma opti_somethin''l : forall l l' a,
+    In a l -> In a (remove_dup_ids l l').
+Proof.
+  induction l; intros.
+  - inv H.
+  - simpl.
+    remember (existsb (fun i => ident_string_beq a i) l') as thing.
+    destruct H.
+    + subst a0.
+      destruct thing.
+      apply opti_somethin''r.
+      rewrite <- in_exists_eq.
+      rewrite Heqthing.
+      reflexivity.
+      apply ident_string_beq_refl.
+      apply ident_string_beq_iff_true.
+      apply opti_somethin''r.
+      left. reflexivity.
+    + destruct thing.
+      apply IHl.
+      assumption.
+      apply IHl.
+      assumption.
+Qed.
+
+Lemma blublub : forall l envv id v,
+  nsLookup ident_string_beq id (gather_values envv l) = Some v ->
+  In id l.
+Proof.
+  induction l; intros.
+  - simpl in *. inv H.
+  - simpl in *.
+    remember (nsLookup ident_string_beq a envv) as eqa.
+    destruct eqa.
+    unfold nsLookup in H.
+    unfold lookup in H.
+    remember (ident_string_beq id a) as ida.
+    destruct ida.
+    symmetry in Heqida.
+    rewrite ident_string_beq_iff_true in Heqida.
+    left. subst. reflexivity.
+    right.
+    eapply IHl.
+    apply H.
+    right.
+    eapply IHl.
+    apply H.
+Qed.
+
+Lemma nsLookup_iff_id_In_env : forall (envv : env_val) id,
+  (exists v, nsLookup ident_string_beq id envv = Some v) <->
+  In id (map fst envv).
+Proof.
+  split.
+  induction envv; simpl in *; intros.
+  - inv H.
+    inv H0.
+  - destruct a.
+    unfold nsLookup in H.
+    simpl in *.
+    remember (ident_string_beq id i ) as idi.
+    destruct idi.
+    symmetry in Heqidi.
+    rewrite ident_string_beq_iff_true in Heqidi.
+    left. subst. reflexivity.
+    right. eapply IHenvv.
+    apply H.
+  - induction envv.
+    intros.
+    inv H.
+    destruct a.
+    intros.
+    simpl in H.
+    destruct H. subst.
+    unfold nsLookup in *; simpl in *.
+    rewrite ident_string_beq_refl.
+    exists v. reflexivity.
+    unfold nsLookup in *; simpl in *.
+    destruct (Namespace.ident_eq_dec _ _ string_dec string_dec id i).
+    subst.
+    rewrite ident_string_beq_refl.
+    exists v. reflexivity.
+    rewrite <- ident_string_beq_iff_false in n.
+    rewrite n.
+    apply IHenvv.
+    assumption.
+Qed.
+
+Lemma blublublublub : forall l (envv : env_val) id v,
+  nsLookup ident_string_beq id (gather_values envv l) = Some v ->
+  In id (map fst envv).
+Proof.
+  induction l; intros.
+  - inv H.
+  - unfold nsLookup in H.
+    simpl in *.
+    remember (nsLookup ident_string_beq a envv) as lookupa.
+    destruct lookupa.
+    simpl in *.
+    remember (ident_string_beq id a) as ida.
+    destruct ida.
+    symmetry in Heqida.
+    rewrite ident_string_beq_iff_true in Heqida.
+    eapply nsLookup_iff_id_In_env.
+    symmetry in Heqlookupa.
+    subst.
+    eexists.
+    apply Heqlookupa.
+    eapply IHl.
+    apply H.
+    eapply IHl.
+    apply H.
+Qed.
+
+Lemma gather_values_empty_namespace : forall l, gather_values [] l = [].
+Proof.
+  induction l; simpl; try reflexivity; try assumption.
+Qed.
+
+
+Lemma idk_yet : forall id envv a l,
+    id <> a ->
+    nsLookup ident_string_beq id (gather_values envv (a :: l)) =
+      nsLookup ident_string_beq id (gather_values envv l).
+Proof.
+  intros.
+  simpl in *.
+  break_match.
+  unfold nsLookup in *; simpl in *.
+  rewrite <- ident_string_beq_iff_false in H.
+  rewrite H.
+  reflexivity.
+  reflexivity.
+Qed.
+
+Lemma eureka : forall id envv l,
+  (exists v, nsLookup ident_string_beq id (gather_values envv l) = Some v) <->
+  In id (map fst envv) /\ In id l.
+Proof.
+  split.
+  split.
+  destruct H.
+  eapply blublublublub. apply H.
+  destruct H.
+  eapply blublub. apply H.
+  intros.
+  generalize dependent envv.
+  generalize dependent l.
+  induction l; intros.
+  - destruct H. inv H0.
+  - destruct H.
+    destruct H0.
+    + subst.
+      rewrite <- nsLookup_iff_id_In_env in H.
+      destruct H.
+      simpl.
+      rewrite H.
+      exists x.
+      unfold nsLookup. simpl.
+      rewrite ident_string_beq_refl.
+      reflexivity.
+    + unfold nsLookup in *; simpl in *.
+      break_match.
+      simpl.
+      break_if.
+      exists v. reflexivity.
+      apply IHl.
+      split; assumption.
+      apply IHl.
+      split; assumption.
+Qed.
+
+Lemma In_gather_In_env :
+  forall l envv id v,
+    In (id,v) (gather_values envv l) -> In id (map fst envv).
+Proof.
+  induction l; intros.
+  - inv H.
+  - simpl in *.
+    break_match.
+    simpl in *.
+    destruct H.
+    subst. simpl.
+    eapply nsLookup_iff_id_In_env.
+    exists v.
+    inv H.
+    assumption.
+    eapply IHl.
+    apply H.
+    eapply IHl.
+    apply H.
+Qed.
+
+Lemma In_gather_In_l :
+  forall l envv id v,
+    In (id,v) (gather_values envv l) -> In id l.
+Proof.
+  induction l; intros.
+  inv H.
+  simpl in *.
+  break_match.
+  simpl in H.
+  destruct H.
+  subst.
+  left. inv H. reflexivity.
+  right. eapply IHl. apply H.
+  right. eapply IHl. apply H.
+Qed.
+
+Theorem wrong : forall l id v envv ,
+    nsLookup ident_string_beq id envv = Some v /\
+    In id l <->
+    In (id,v) (gather_values envv l).
+Proof.
+  split;
+    revert l envv.
+  - induction l; intros.
+    + destruct H. inv H0.
+    + simpl in *.
+      destruct H.
+      destruct H0. subst.
+      rewrite H.
+      simpl.
+      left; reflexivity.
+      simpl in *.
+      break_match.
+      simpl.
+      right.
+      apply IHl.
+      split; assumption.
+      apply IHl.
+      split; assumption.
+  - induction l; intros.
+    + inv H.
+    + split.
+      simpl in *.
+      break_match.
+      destruct H.
+      inv H.
+      assumption.
+      apply IHl in H. destruct H. assumption.
+      apply IHl in H. destruct H. assumption.
+      simpl in *.
+      break_match.
+      destruct H.
+      inv H.
+      left; reflexivity.
+      right.
+      apply IHl in H. destruct H. assumption.
+      right.
+      apply IHl in H. destruct H. assumption.
+Qed.
+
+Ltac copy H :=
+  match type of H with
+  | ?anything =>
+      assert anything by apply H
+  end.
+
+Ltac andtogether H H' :=
+  match type of H with
+  | ?anything =>
+      match type of H' with
+      | ?anything' => assert (anything /\ anything') by (split; assumption)
+      end
+  end.
+
+Lemma In_remove_true : forall l x, In x (remove_dup_ids l [x]).
+Proof.
+  induction l; intros.
+  - left. reflexivity.
+  - apply opti_somethin''r.
+    left. reflexivity.
+Qed.
+
+Definition id_dec x y := Namespace.ident_eq_dec _ _ string_dec string_dec x y.
+
+Lemma idk : forall l x l', ~ In x l' ->
+            In x (remove_dup_ids l l') ->
+            In x l.
+Proof.
+  induction l; intros.
+  simpl in *.
+  contradiction H.
+  simpl in *.
+  break_if.
+  rewrite in_exists_eq in Heqb.
+  right.
+  eapply IHl.
+  apply H.
+  assumption.
+  apply ident_string_beq_refl.
+  apply ident_string_beq_iff_true.
+  rewrite not_in_exists_eq in Heqb.
+  Check idk_still.
+  destruct (id_dec x a).
+  subst.
+  left; reflexivity.
+  right.
+  assert (~ In x (a::l')).
+  intro contra. simpl in contra.
+  destruct contra.
+  contradiction n.
+  auto.
+  contradiction H.
+  eapply IHl.
+  apply H1.
+  assumption.
+  apply ident_string_beq_refl.
+  apply ident_string_beq_iff_false.
+Qed.
+
+Lemma idk' : forall l x, In x (remove_dup_ids l []) -> In x l.
+Proof.
+  induction l; intros.
+  inv H.
+
+  destruct (id_dec a x).
+  left. auto.
+  apply idk with [].
+  intro contra.
+  inv contra.
+  assumption.
+Qed.
+
+Lemma simple_remove_dup : forall x l, In x l <-> In x (remove_dup_ids l []).
+Proof.
+  induction l;
+    split; intros.
+  - inv H.
+  - inv H.
+  - destruct H.
+    + subst.
+      apply In_remove_true.
+    + simpl.
+      destruct (id_dec x a).
+      subst.
+      apply In_remove_true.
+      apply opti_somethin''l.
+      assumption.
+  - apply idk'.
+    assumption.
+Qed.
+
+Lemma In_gather_entails_lookup_val : forall l a v envv,
+    In (a, v) (gather_values envv l) ->
+    nsLookup ident_string_beq a envv = Some v.
+Proof.
+  induction l; intros.
+  - inv H.
+  - simpl in *.
+    break_match.
+    simpl in *.
+    destruct H.
+    inv H.
+    assumption.
+    apply IHl.
+    assumption.
+    apply IHl.
+    assumption.
+Qed.
+
+Lemma In_gather_entails_lookup_gather : forall l a v envv,
+    In (a, v) (gather_values envv l) ->
+    nsLookup ident_string_beq a (gather_values envv l) = Some v.
+Proof.
+  intros.
+  copy H.
+  apply In_gather_entails_lookup_val in H0.
+  unfold nsLookup in *.
+  simpl in *.
+  generalize dependent a.
+  revert l envv v.
+  induction l; intros.
+  - inv H.
+  - simpl in *.
+    break_match.
+    simpl in *.
+    destruct H.
+    inv H.
+    rewrite ident_string_beq_refl.
+    reflexivity.
+    simpl in *.
+    break_if.
+    rewrite ident_string_beq_iff_true in Heqb; subst.
+    rewrite <- Heqo.
+    rewrite <- H0.
+    reflexivity.
+    apply IHl. assumption.
+    assumption.
+    apply IHl; try assumption.
+Qed.
+
+Lemma In_gather_iff_In_gather_remove_l : forall l p envv,
+  In p (gather_values envv l) <->
+    In p (gather_values envv (remove_dup_ids l [])).
+Proof.
+  split; revert l envv p.
+  - induction l; intros.
+    + inv H.
+    + destruct p.
+      copy H.
+      copy H.
+      apply wrong in H.
+      apply wrong.
+      split.
+      destruct H. assumption.
+      apply opti_somethin''l.
+      destruct H.
+      assumption.
+  - induction l; intros.
+    + inv H.
+    + destruct p.
+      apply wrong.
+      copy H.
+      apply In_gather_In_l in H.
+      rewrite <- simple_remove_dup in H.
+      split; try assumption.
+      destruct (id_dec i a); subst.
+      eapply In_gather_entails_lookup_val.
+      apply H0.
+      eapply In_gather_entails_lookup_val.
+      apply H0.
+Qed.
+
+Lemma eureka' : forall (id : ident tvarN tvarN) (envv : namespace tvarN tvarN val)
+                  (l : list (ident tvarN tvarN)) v,
+    nsLookup ident_string_beq id (gather_values envv l) = Some v ->
+    In id (map fst envv) /\ In id l.
+Proof.
+  intros.
+  apply eureka.
+  exists v.
+  assumption.
+Qed.
+
+Lemma eureka'' : forall l id envv v,
+    nsLookup ident_string_beq id (gather_values envv l) = Some v ->
+    In (id,v) (gather_values envv l).
+Proof.
+  induction l; intros.
+  - inv H.
+
+  - simpl in *.
+    break_match.
+    unfold nsLookup in *.
+    simpl in *.
+    break_if.
+    rewrite ident_string_beq_iff_true in Heqb; subst.
+    inv H.
+    left; reflexivity.
+    right.
+    apply IHl.
+    assumption.
+    apply IHl.
+    assumption.
+Qed.
+
+
+Lemma opti_somethin'' : forall l id envv v,
+    nsLookup ident_string_beq id (gather_values envv l) = Some v ->
+    nsLookup ident_string_beq id (gather_values envv (remove_dup_ids l [])) = Some v.
+Proof.
+  induction l; intros.
+  - inv H.
+  - destruct (Namespace.ident_eq_dec _ _ string_dec string_dec id a); subst.
+    Check idk_yet.
+    Check wrong.
+    copy H.
+    apply eureka' in H.
+    destruct H.
+    Check wrong.
+    simpl in H0.
+    break_match.
+    copy H0.
+    simpl in H2.
+    unfold nsLookup in H2.
+    simpl in H2.
+    rewrite ident_string_beq_refl in H2.
+    inv H2.
+    Check idk_still.
+    Check In_gather_iff_In_gather_remove_l.
+    Check eureka'.
+    apply In_gather_entails_lookup_gather.
+    rewrite <- In_gather_iff_In_gather_remove_l.
+    simpl.
+    rewrite Heqo.
+    left. reflexivity.
+    apply In_gather_entails_lookup_gather.
+    rewrite <- In_gather_iff_In_gather_remove_l.
+    simpl.
+    rewrite Heqo.
+    apply eureka''.
+    assumption.
+    copy H.
+    apply eureka' in H.
+    destruct H.
+    Check wrong.
+    apply In_gather_entails_lookup_gather.
+    rewrite <- In_gather_iff_In_gather_remove_l.
+    apply eureka''.
+    assumption.
+Qed.
+
+Theorem idk_yet' : forall e id env v,
+    In id (free_vars e []) ->
+    nsLookup ident_string_beq id (sev env) = Some v ->
+    nsLookup ident_string_beq id (sev (optimize_recclosure_env e env)) = Some v.
+Proof.
+  unfold optimize_recclosure_env; simpl.
+  intros. apply opti_somethin''.
+    apply In_gather_entails_lookup_gather.
+    Check eureka.
+    apply wrong.
+    split; try assumption.
+Qed.
+
+Check evaluate.
+Theorem idk_fuck_me_Ihatemyselfwhycantisolvethisstupidproblemfuckfuckfuck :
+  forall e f st (env : sem_env val),
+    evaluate [e] f st env =
+      evaluate [e] f st (optimize_recclosure_env e env).
+Proof.
+  unfold evaluate.
+  induction e; intros.
+  - simp eval_or_match in *.
+    rewrite IHe.
+    unfold optimize_recclosure_env.
+    simpl.
+    reflexivity.
+  - induction X.
+    + simp eval_or_match; simpl.
+      unfold optimize_recclosure_env in *.
+      unfold update_sev in *.
+      simpl.
+      rewrite app_nil_r.
+      unfold update_sev.
+      rewrite IHe.
+      unfold eval_or_match_unfold_clause_4.
+      break_match.
+      break_match.
+      reflexivity.
+      break_match.
+      simp eval_or_match.
+      reflexivity.
+      reflexivity.
+    + destruct x.
+      simpl in *.
+      clear X.
+      simp eval_or_match; simpl.
+      simp eval_or_match in IHX; simpl in IHX.
+      unfold eval_or_match_unfold_clause_4 in *.
+      break_match.
+      break_match.
+      unfold optimize_recclosure_env, update_sev in *.
+      (* HERE *)
+
+
+      break_match.
+      break_match.
+      break_match.
+      break_match.
+      subst.
+      Admitted.
+
+
+
+
+
+Theorem EVAL_optimize_ELetrec :
+  forall (A B : Type) (env : sem_env val) (AINV : A -> val -> Prop) (BINV : B -> val -> Prop) (f : A -> B) (fname var : varN) (body : exp),
+    EVAL env (ELetrec [(fname,var,body)] (EVar (Short fname))) ((FUNC AINV BINV) f) ->
+    EVAL (optimize_recclosure_env body env) (ELetrec [(fname,var,body)] (EVar (Short fname))) ((FUNC AINV BINV) f).
+Proof.
+  unfold EVAL, evaluate.
+  intros.
+  specialize (H st).
+  destruct H as [v [fH [st' [Heval Hinv]]]].
+  do 3 eexists.
+  simp eval_or_match in *; simpl in *.
+  unfold build_rec_env in *; simpl in *.
+  unfold nsLookup in *; simpl in *.
+  unfold update_sev in *; simpl in *.
+  unfold nsBind in *; simpl in *.
+  break_if.
+  simpl in *.
+  split.
+  reflexivity.
+  unfold FUNC in *.
+  intros.
+  specialize (Hinv x v0 H).
+  destruct Hinv as [u [HBinvu Happ_returns]].
+  exists u.
+  split.
+  assumption.
+  unfold app_returns in *.
+  intros.
+  specialize (Happ_returns v1 H0 st0).
+  destruct Happ_returns as [Henv [Hexp [Hst [Hu [Hdoapp [Heval_rel HBinvu']]]]]].
+  inv Heval.
+  eexists.
+  unfold do_opapp in *.
+  break_if.
+  simpl in *.
+  exists body, Hst, Hu.
+  break_if.
+  unfold update_sev.
+  unfold build_rec_env.
+  simpl.
+  unfold nsBind.
+  split.
+  reflexivity.
+  unfold eval_rel in *.
+  unfold evaluate in *.
+  destruct Heval_rel as [Hf Heval_rel].
+  inv Hdoapp.
+  unfold update_sev, nsBind, build_rec_env in *. simpl in *.
+  split; try assumption.
+  exists Hf.
+  clear H H0 Hdoapp Heval HBinvu HBinvu' v0 Heqb0.
+  revert Heval_rel.
+  revert Hf st0 Hst Hu.
+  induction Hexp; intros.
+  intros.
+  simp eval_or_match in *; simpl in *.
+  unfold optimize_recclosure_env in *.
+  unfold update_sev in *.
+  simpl in *.
+Admitted.
